code/mpfr/MPFR.Lib.Spec.fst
@@ -6,112 +6,139 @@ open MPFR.Maths
 
 #set-options "--z3refresh --z3rlimit 5 --max_fuel 1 --initial_fuel 0 --max_ifuel 1 --initial_ifuel 0"
 
+(* MPFR uses 'mpfr_sign', 'mpfr_prec', 'mpfr_exp' and 'mpfr_d' to describe a dyadic rational number,
+ * it also allows "sigular" values for NaN, +-Inf and +-ZERO.
+ * for regular values, aka non-zero values,
+ * 'mpfr_d' is an array of uint64 represents the significand in the following way:
+ * it should start with bit '1' and the last certain bits (depends on precision) should be '0's
+ * thus it represent a number in [0.5, 1) by adding '0.' in front of it.
+ * Therefore, the whole mpfr_struct should represent a value:
+ *             mpfr_sign * mpfr_d * 2^mpfr_exp.
+ * In this file a struct is defined to store MPFR format floating point number. *)
+
 
 ///////////////////////////////////////////////////////
 //  Struct Definition                                //
-//  Used to store IEEE format floating point number  //
+//  Used to store MPFR format floating point number  //
 ///////////////////////////////////////////////////////
 
-(* MPFR uses 'mpfr_sign', 'mpfr_prec', 'mpfr_exp' and 'mpfr_d' to describe a dyadic rational number
- * 'mpfr_d' is an array of uint64 represent the mantissa in the following way:
- * it should start with bit '1' and the last certain bits (depends on precision) should be '0's
- * thus it represent a number in [0.5, 1) by adding '0.' in front of it.
- * This struct is going to follow similar rules:
- * 'sign', 'prec' and 'exp' give the sign, precision and exponent of the number resprectively
- * 'limb' is a 'len'-bit natural number (possibly with leading zeros) represents the significand *)
+(* indicating regular/sigular value type *)
+type fp_type_t =
+   | MPFR_NUM      (* regular number (excludes zero) *)
+   | MPFR_ZERO     (* +0 or -0                       *)
+   | MPFR_INF      (* +inf or -inf                   *)
+   | MPFR_NAN      (* not a number                   *)
+   
+(* flag: indicates value type, other entries are useless for sigular value (except sign)
+ * sign: sign of the value, indicates also the sign of zero and infinity
+ * prec: precision of the value, see more information below with limb
+ * exp : exponent of the value
+ * len : the bit length of significand, see more information below with limb
+ * limb: significand of the value, it is a 'len'-bit natural number (possibly with leading zeros),
+         the first 'prec' bits can have values while the last 'len - prec' bits should be 0s.
+	 it represents a rational number between 0 and 1 by adding '0.' in front of it *)
 type fp_struct = {
     sign: s:int{s = -1 \/ s = 1};
     prec: pos;
     exp : int;
     limb: nat;
     len : pos;
+    flag: fp_type_t
 }
 
-let mk_struct sign prec exp limb len = {
+(* constructor *)
+let mk_struct sign prec exp limb len flag = {
     sign = sign;
     prec = prec;
     exp  = exp;
     limb = limb;
-    len  = len
+    len  = len;
+    flag = flag
 }
 
-(* Get bit length of a positive integer *)
-val nb_of_bits: m:pos -> Tot (p:pos{pow2 (p - 1) <= m /\ m < pow2 p})
-let nb_of_bits m = log2 m + 1
 
-val nb_of_bits_lemma: m:pos -> p:pos{pow2 (p - 1) <= m /\ m < pow2 p} ->
-    Lemma (nb_of_bits m = p)
-let nb_of_bits_lemma m p =
-    lemma_log2_le (pow2 (p - 1)) m;
-    lemma_log2_lt m p
+///////////////////////////////////////////////////////////////////////////////////////////
+//  Evaluation for the struct                                                            //
+//  Only regular numbers and +-0 can be evaluated to a dyadic                            //
+//  The precision should be positive and not greater than the bit length of significand  //
+//  Also the last 'len - prec' bits should be 0s                                         //
+///////////////////////////////////////////////////////////////////////////////////////////
 
-type valid_struct = s:fp_struct{s.limb = 0 \/ nb_of_bits s.limb <= s.len}
+(* validity for zero *)
+let valid_zero_cond s = MPFR_ZERO? s.flag /\ s.limb = 0
 
-(* Evaluation. Here is the method.
- * Firstly add '0.' in front of 'limb' to make it a floating number in (0, 1)
- * Then multiply it with 2 ^ exp *)
-let eval (fp:valid_struct) = mk_fp (fp.sign * fp.limb) (fp.exp - fp.len)
-
-
-/////////////////////////////////////////////////////////////////////////////////////////
-//  Validity Test for ieee_struct                                                      //
-//  A valid struct represents a binary floating point number defined in MPFR.BinaryFP  //
-//  Important function 'eval' maps ieee_fp to dyadic                                   //
-/////////////////////////////////////////////////////////////////////////////////////////
-
-(* Condition for validity 
- * A valid struct should have a positive precision which is smaller than 'limb' length
- * Only the first 'prec' bits of 'limb' store value and the rest bits are 0s *)
-let ieee_valid_cond (s:fp_struct) =
-    s.limb > 0 /\ nb_of_bits s.limb = s.len /\
+(* validity for non-zero *)
+let valid_num_cond s =
+    MPFR_NUM? s.flag /\ 0 < s.limb /\ s.limb < pow2 s.len /\
     0 < s.prec /\ s.prec <= s.len /\
     s.limb % pow2 (s.len - s.prec) = 0
-    
-type ieee_fp = s:valid_struct{ieee_valid_cond s}
 
-let mk_ieee sign prec exp limb len: Pure ieee_fp
-    (requires (ieee_valid_cond (mk_struct sign prec exp limb len)))
+(* validity for evaluation *)
+let valid_fp_cond s = valid_zero_cond s \/ valid_num_cond s
+
+(* type for fp_struct which can be evaluated *)
+type valid_fp = s:fp_struct{valid_fp_cond s}
+
+(* Evaluation.
+ * Firstly add '0.' in front of 'limb' to make it a floating number in (0, 1)
+ * Then multiply it with 2 ^ exp *)
+let eval (fp:valid_fp) = mk_fp (fp.sign * fp.limb) (fp.exp - fp.len)
+
+
+//////////////////////////////////////////////////////////////////////
+//  Normalize a regular value                                       //
+//  A regular value is called normal when there's no leading zeros  //
+//////////////////////////////////////////////////////////////////////
+
+(* validity for normal number *)
+let normal_fp_cond (s:valid_fp) = valid_num_cond s /\ s.limb >= pow2 (s.len - 1)
+
+(* type for normal number *)
+type normal_fp = s:valid_fp{normal_fp_cond s}
+
+(* constructor for normal number *)
+let mk_normal sign prec exp limb len flag: Pure normal_fp
+    (requires (valid_fp_cond  (mk_struct sign prec exp limb len flag) /\
+              normal_fp_cond (mk_struct sign prec exp limb len flag)))
     (ensures  (fun _ -> True)) =
-    mk_struct sign prec exp limb len
+    mk_struct sign prec exp limb len flag
 
 
-//////////////////////////////////////////////////////
-//  A special type corresponding to top level code  //
-//  Pure version of mpfr_struct                     //
-//////////////////////////////////////////////////////
+////////////////////////////////////////////////////////////////////////////////
+//  Pure version of mpfr_struct                                               //
+//  A MPFR number has limits for its precision and exponent                   //
+//  The bit length of limb must be a multiple of 64 and as small as possible  //
+////////////////////////////////////////////////////////////////////////////////
 
-(* Condition for parameters range corresponding to top level code *)
-let gmp_NUMB_BITS = 64
-let mpfr_PREC_MIN = 1
-let mpfr_PREC_MAX = pow2 31 - 1
-let mpfr_PREC_COND (p:nat) = mpfr_PREC_MIN <= p /\ p <= mpfr_PREC_MAX
+(* range limits for precision and exponent *)
+let mpfr_PREC_COND (p:pos) = p < pow2 31
 
-let mpfr_EXP_INVALID = pow2 30
-let mpfr_EMIN = 1 - mpfr_EXP_INVALID
-let mpfr_EMAX = mpfr_EXP_INVALID - 1
-let mpfr_EXP_COND (x:int) = mpfr_EMIN <= x /\ x <= mpfr_EMAX
+let mpfr_EXP_COND  (x:int) = -pow2 30 < x /\ x < pow2 30
 
-(* Condition for a MPFR floating number
- * The precision and exponent have range limits
- * The bit length of limb must be a multiple of 64 and as small as possible *)
-val arr_size: p:pos ->
+(* Get len from prec for a MPFR number *)
+val prec_to_len: p:pos ->
     Tot (s:pos{s % 64 = 0 /\ s >= p /\ s - 64 < p})
-let arr_size p = ((p + 63) / 64) * 64
+let prec_to_len p = ((p + 63) / 64) * 64
 
-val arr_size_lemma: p:pos -> s:pos{s % 64 = 0 /\ s >= p /\ s - 64 < p} ->
-    Lemma (arr_size p = s)
-let arr_size_lemma p s =
+val prec_to_len_lemma: p:pos -> s:pos{s % 64 = 0 /\ s >= p /\ s - 64 < p} ->
+    Lemma (prec_to_len p = s)
+let prec_to_len_lemma p s =
     lemma_div_le (p + 63) (s + 63) 64;
-    //lemma_div_distr s 63 64;
-    //! assert((p + 63) / 64 <= s);
-    lemma_div_le s (p + 63) 64;
-    //lemma_multiple_div s 64;
-    //! assert(s <= (p + 63) / 64);
-    ()
+    lemma_div_le s (p + 63) 64
 
-let mpfr_valid_cond (s:ieee_fp) =
-    s.len = arr_size s.prec /\
+(* validity for normal number of MPFR *)
+let mpfr_reg_fp_cond (s:normal_fp) =
+    s.len = prec_to_len s.prec /\
     mpfr_PREC_COND s.prec /\
     mpfr_EXP_COND s.exp
 
-type mpfr_fp = f:ieee_fp{mpfr_valid_cond f}
+(* type for normal number of MPFR *)
+type mpfr_reg_fp = f:normal_fp{mpfr_reg_fp_cond f}
+
+(* validity for MPFR number allowing sigular values *)
+let mpfr_fp_cond (s:fp_struct) =
+    MPFR_NAN? s.flag \/ MPFR_INF? s.flag \/ valid_zero_cond s \/ 
+    (valid_fp_cond s /\ normal_fp_cond s /\ mpfr_reg_fp_cond s)
+
+(* type for MPFR number *)
+type mpfr_fp = s:fp_struct{mpfr_fp_cond s}
