code/mpfr/MPFR.Lib.fst
@@ -32,13 +32,15 @@ let mpfr_EXP_INVALID = assert_norm(0x40000000 = pow2 30); 0x40000000l
 let mpfr_EMIN = I32.(1l -^ mpfr_EXP_INVALID)
 let mpfr_EMAX = I32.(mpfr_EXP_INVALID -^ 1l)
 
-type mpfr_sign_t = s:i32{I32.(s = -1l \/ s = 1l)}
-type mpfr_prec_t = p:u32{mpfr_PREC_COND (U32.v p)}
-type mpfr_exp_t  = x:i32{mpfr_EXP_COND  (I32.v x)}
-type mpfr_uexp_t = u32
+type mpfr_sign_t = s:i32{s = mpfr_SIGN_NEG \/ s = mpfr_SIGN_POS}
 type mp_limb_t = u64
+type mpfr_prec_t = u32
+type mpfr_exp_t  = i32
+type mpfr_prec_vt = p:mpfr_prec_t{mpfr_PREC_COND (U32.v p)}
+type mpfr_exp_vt  = x:mpfr_exp_t{mpfr_EXP_COND (I32.v x)}
 
-let neg (x:mpfr_sign_t) = if x = 1l then -1l else 1l
+let neg_sign (x:mpfr_sign_t) = if x = 1l then -1l else 1l
+
 
 noeq type mpfr_struct = {
     mpfr_prec: mpfr_prec_t;
@@ -48,15 +50,18 @@ noeq type mpfr_struct = {
 }
 
 (* First bit is 1 *)
-let mpfr_d_val0_cond (m:mp_limb_t): Type = v m >= pow2 63
+let mpfr_d_val0_cond (m:mp_limb_t): Type =
+    v m >= pow2 63
 (* Ending bits are 0 *)
-let mpfr_d_valn_cond (m:mp_limb_t) (p:mpfr_prec_t): Type = v m % pow2 (arr_size (U32.v p) - U32.v p) = 0
+let mpfr_d_valn_cond (m:mp_limb_t) (p:mpfr_prec_vt): Type =
+    v m % pow2 (prec_to_len (U32.v p) - U32.v p) = 0
 
 let valid_mpfr_struct h (s:mpfr_struct): Type =
-    let l = length s.mpfr_d in
+    mpfr_PREC_COND (U32.v s.mpfr_prec) /\ mpfr_EXP_COND (I32.v s.mpfr_exp) /\
+    (let l = length s.mpfr_d in
     l >= 1 /\ (l - 1) * 64 < U32.v s.mpfr_prec /\ U32.v s.mpfr_prec <= l * 64 /\
     mpfr_d_val0_cond (get h s.mpfr_d 0) /\
-    mpfr_d_valn_cond (get h s.mpfr_d (l - 1)) s.mpfr_prec
+    mpfr_d_valn_cond (get h s.mpfr_d (l - 1)) s.mpfr_prec)
 
 (* Conversion to pure struct *)
 val to_val: s:Seq.seq u64 -> Tot (n:nat{n < pow2 (Seq.length s * 64)}) (decreases (Seq.length s))
@@ -79,18 +84,18 @@ let val0_cond_lemma s =
     lemma_pow2_mul 63 ((Seq.length s - 1) * 64);
     lemma_pow2_le (Seq.length s * 64 - 1) (63 + (Seq.length s - 1) * 64)
 
-val valn_cond_lemma: s:Seq.seq u64 -> p:mpfr_prec_t{arr_size (U32.v p) = Seq.length s * 64} -> Lemma
+val valn_cond_lemma: s:Seq.seq u64 -> p:mpfr_prec_vt{prec_to_len (U32.v p) = Seq.length s * 64} -> Lemma
     (requires  (Seq.length s > 0 /\ mpfr_d_valn_cond (Seq.index s (Seq.length s - 1)) p))
     (ensures   (to_val s % pow2 (Seq.length s * 64 - U32.v p) = 0))
     (decreases (U32.v p))
     
 let rec valn_cond_lemma s p = 
     admit(); (* It takes very long to go throught, need more robust proof *)
-    if U32.v p <= 64 then arr_size_lemma (U32.v p) 64 else begin
+    if U32.v p <= 64 then prec_to_len_lemma (U32.v p) 64 else begin
         lemma_pow2_mul ((Seq.length s - 1) * 64 - (Seq.length s) * 64 + U32.v p) ((Seq.length s) * 64 - U32.v p);
         lemma_multiple_mod (v (Seq.index s 0) * pow2 ((Seq.length s - 1) * 64 - Seq.length s * 64 + U32.v p)) (pow2 (Seq.length s * 64 - U32.v p));
         assert((v (Seq.index s 0) * pow2 ((Seq.length s - 1) * 64)) % pow2 (Seq.length s * 64 - U32.v p) = 0);
-	arr_size_lemma (U32.v p - 64) ((Seq.length s - 1) * 64);
+	prec_to_len_lemma (U32.v p - 64) ((Seq.length s - 1) * 64);
 	valn_cond_lemma (Seq.slice s 1 (Seq.length s)) (U32.(p -^ 64ul));
 	assert(to_val (Seq.slice s 1 (Seq.length s)) % pow2 (Seq.length s * 64 - U32.v p) = 0);
         to_val_rec_lemma s;
@@ -113,14 +118,14 @@ let as_pure h s =
     let exp  = I32.v s.mpfr_exp  in
     let limb = as_val h s.mpfr_d in
     let l    = length s.mpfr_d in
-    arr_size_lemma prec (l * 64);
+    prec_to_len_lemma prec (l * 64);
     //! assert(arr_size prec = l * 64);
     val0_cond_lemma (as_seq h s.mpfr_d);
     //! assert(limb >= pow2 (l * 64 - 1));
     nb_of_bits_lemma limb (l * 64);
     //! assert(nb_of_bits limb = l * 64);
     valn_cond_lemma (as_seq h s.mpfr_d) s.mpfr_prec;
-    mk_ieee sign prec exp limb (l * 64)
+    mk_struct sign prec exp limb (l * 64)
 
 (* Struct functions *)
 type mpfr_ptr = b:buffer mpfr_struct{length b = 1}
@@ -135,17 +140,17 @@ let mk_mpfr_struct p s e d = {
 val mpfr_SIGN: x:mpfr_ptr -> Stack mpfr_sign_t 
 		(requires (fun h -> live h x))
 		(ensures (fun h0 r h1 -> live h1 x /\ h0 == h1 /\
-		            (let xm = Seq.index (as_seq h0 x) 0 in
-			     r == xm.mpfr_sign)))
+		            (let xm = Seq.index (as_seq h1 x) 0 in
+			     r = xm.mpfr_sign)))
 let mpfr_SIGN x = 
     let f = x.(0ul) in
     f.mpfr_sign
 
 val mpfr_EXP: x:mpfr_ptr -> Stack mpfr_exp_t 
 		(requires (fun h -> live h x))
-		(ensures (fun h0 r h1 -> live h1 x /\ h0 == h1 /\
-			    (let xm = Seq.index (as_seq h0 x) 0 in
-			     r == xm.mpfr_exp)))
+		(ensures  (fun h0 r h1 -> live h1 x /\ h0 == h1 /\
+			      (let xm = Seq.index (as_seq h1 x) 0 in
+			      r = xm.mpfr_exp)))
 let mpfr_EXP x = 
     let f = x.(0ul) in
     f.mpfr_exp
@@ -154,9 +159,12 @@ let mpfr_GET_EXP x = mpfr_EXP x
 
 val mpfr_SET_EXP: x:mpfr_ptr -> e:mpfr_exp_t -> Stack unit
 		(requires (fun h -> live h x))
-		(ensures (fun h0 _ h1 -> live h1 x /\ modifies_1 x h0 h1 /\
-			    (let xm = Seq.index (as_seq h1 x) 0 in
-			     e == xm.mpfr_exp)))
+		(ensures  (fun h0 _ h1 -> live h1 x /\ modifies_1 x h0 h1 /\
+			      (let xm0 = Seq.index (as_seq h0 x) 0 in
+			      let xm = Seq.index (as_seq h1 x) 0 in
+			      xm0.mpfr_sign = xm.mpfr_sign /\
+			      xm0.mpfr_prec = xm.mpfr_prec /\
+			      xm0.mpfr_d == xm.mpfr_d /\ e = xm.mpfr_exp)))
 let mpfr_SET_EXP x e = 
     let f = x.(0ul) in
     x.(0ul) <- {f with mpfr_exp = e}
@@ -165,7 +173,7 @@ let mpfr_SET_EXP x e =
 val mpfr_MANT: x:mpfr_ptr -> Stack (buffer mp_limb_t)
 		(requires (fun h -> live h x))
 		(ensures (fun h0 r h1 -> live h1 x /\ h0 == h1 /\
-			    (let xm = Seq.index (as_seq h0 x) 0 in
+			    (let xm = Seq.index (as_seq h1 x) 0 in
 			     r == xm.mpfr_d)))
 let mpfr_MANT x = 
     let f = x.(0ul) in
